% -*- coding:utf-8 -*-
\documentclass[12pt]{article}
\usepackage[utf8]{inputenc}
\newenvironment{note}{\paragraph{NOTE:}}{}
\newenvironment{field}{\paragraph{field:}}{}
\begin{document}
\section{Meteorites-Radiation}
\begin{note}
   \begin{field}
        Given \(N_p(t)=e^{-\frac{t-t_0}{\tau_m}}N_p(t_0)\), derive \(N_d(t)\).
   \end{field}
   \begin{field}
   		\[
   			N_p(t)=e^{-\frac{t-t_0}{\tau_m}}N_p(t_0)
   		\]
   		\[
   			N_d(t)=N_d(t_0)+(N_p(t_0)-N_p(t))
   		\]
   		\[
   			N_d(t)=N_d(t_0)+(N_p(t_0)-e^{-\frac{t-t_0}{\tau_m}}N_p(t_0))
   		\]
   		\[
   			N_d(t)=N_d(t_0)+N_p(t_0)(1-e^{-\frac{t-t_0}{\tau_m}})
   		\]
   		Substitute: \(N_p(t_0)=N_p(t)e^{\frac{t-t_0}{\tau_m}}\):
   		\[
   			N_d(t)=N_d(t_0)+N_p(t)e^{\frac{t-t_0}{\tau_m}}(1-e^{-\frac{t-t_0}{\tau_m}})
   		\]
   		\[
   			N_d(t)=N_d(t_0)+N_p(t)e^{\frac{t-t_0}{\tau_m}}-N_p(t)e^{\frac{t-t_0}{\tau_m}}e^{-\frac{t-t_0}{\tau_m}}
   		\]
   		\[
   			N_d(t)=N_d(t_0)+N_p(t)e^{\frac{t-t_0}{\tau_m}}-N_p(t)
   		\]
   		\[
   			N_d(t)=N_d(t_0)+N_p(t)(e^{\frac{t-t_0}{\tau_m}}-1)
   		\]
   \end{field}
\end{note}
\end{document}